### 证明下列公式
#### a. $\sum_{i=1}^{N}(2i-1)$ = $N_{2}$
$\sum_{i=1}^{N}$(2i-1) = 2 $\sum_{i=1}^N$ i - $\sum_{i=1}^{N}$ 1 = N(N+1)-N = $N^{2}$
#### b. $\sum_{i=1}^{N}$ $i^{3}$ = ($\sum_{i=1}^{N}$ i$)^{2}$
最简单的方法是通过数学归纳法证明。N=1的情况显然成立。其他情况，<br />
$\sum_{i=1}^{N+1}$ $i^{3}$ = (N + 1$)^{3}$ + $\sum_{i=1}^{N}$ $i^{3}$ <br />
= (N + 1$)^{3}$ + $\frac{N^{2}(N + 1)^{2}}{4}$ <br />
= (N + 1$)^{2}$ [$\frac{N^{2}}{4}$ + (N + 1)] <br />
= (N + 1$)^{2}$ [$\frac{N^{2} + 4N + 4}{4}$] <br />
= $\frac{(N + 1)^{2}(N + 2)^{2}}{2^{2}}$ <br />
= $[\frac{(N + 1)(N + 2)}{2}]^{2}$ <br />
= $(\sum_{i=1}^{N+1} i)^{2}$